kami-rv32im: started fixing broken proofs; fixed [procDec_inv_ok] that involves correctness of program init.

Kami/Ex/ProcDecInv.v
@@ -1,4 +1,4 @@
-Require Import Bool String List.
+Require Import Bool String List BinNums Omega.
 Require Import Lib.CommonTactics Lib.ilist Lib.Word.
 Require Import Lib.Struct Lib.FMap Lib.StringEq Lib.Indexer.
 Require Import Kami.Syntax Kami.Semantics Kami.RefinementFacts Kami.Renaming Kami.Wf.
@@ -8,6 +8,51 @@ Require Import Ex.MemTypes Ex.SC Ex.NativeFifo Ex.MemAsync Ex.ProcDec Ex.ProcDec
 Require Import Eqdep ProofIrrelevance.
 
 Set Implicit Arguments.
+
+Lemma wnot_not_zero_wplusone:
+  forall {sz} (w2: word sz),
+    wnot w2 <> $0 ->
+    #(w2 ^+ $1) = #w2 + 1.
+Proof.
+  intros.
+  assert (w2 < wones _).
+  { apply lt_wlt.
+    rewrite wones_pow2_minus_one.
+    pose proof (wordToNat_bound w2).
+    pose proof (NatLib.pow2_zero sz).
+    assert (#w2 = NatLib.pow2 sz - 1 \/ (#w2 < NatLib.pow2 sz - 1)%nat) by omega.
+    destruct H2; [|assumption].
+    assert (natToWord sz (#w2) = natToWord sz (NatLib.pow2 sz - 1)) by congruence.
+    rewrite natToWord_wordToNat, <-wones_natToWord in H3; subst.
+    rewrite wnot_ones in H.
+    exfalso; auto.
+  }
+  erewrite wordToNat_plusone; [|eassumption].
+  omega.
+Qed.
+
+Lemma wminus_wplus_transpose:
+  forall {sz} (w1 w2 w3: word sz),
+    w1 ^- w2 = w3 -> w1 = w3 ^+ w2.
+Proof.
+  intros.
+  replace (w3 ^+ w2) with (w1 ^- w2 ^+ w2).
+  - rewrite wminus_def, <-wplus_assoc.
+    rewrite wplus_comm with (x:= ^~ w2), wminus_inv.
+    rewrite wplus_wzero_1; reflexivity.
+  - congruence.
+Qed.
+
+Lemma wnot_zero_wones:
+  forall {sz} (w: word sz), wnot w = $0 -> w = wones _.
+Proof.
+  intros.
+  rewrite wneg_wnot in H.
+  apply wminus_wplus_transpose in H.
+  rewrite wplus_unit in H.
+  rewrite <-wneg_idempotent with (w0:= w), H.
+  apply eq_sym, wones_wneg_one.
+Qed.
 
 Section Invariants.
   Variables addrSize iaddrSize fifoSize instBytes dataBytes rfIdx: nat.
@@ -22,6 +67,29 @@ Section Invariants.
   Variable (init: ProcInit iaddrSize dataBytes rfIdx).
 
   Definition pdecInl := pdecInl fifoSize fetch dec exec init.
+
+  Definition fifoLength (emptyv fullv: bool)
+             (enqpv deqpv: type (Bit fifoSize)) :=
+    if emptyv then 0
+    else if fullv then NatLib.pow2 fifoSize
+         else #(enqpv ^- deqpv).
+
+  Definition fifo_inv (emptyv fullv: bool)
+             (enqpv deqpv: type (Bit fifoSize)): Prop :=
+    (emptyv || fullv = true <-> enqpv = deqpv).
+
+  Definition fifo_rq_rs_inv
+             (pinitRqv: type Bool)
+             (pinitRqOfsv pinitRsOfsv: type (Bit iaddrSize))
+             (iemptyv ifullv oemptyv ofullv: type Bool)
+             (ienqpv ideqpv oenqpv odeqpv: type (Bit fifoSize)) :=
+    fifo_inv iemptyv ifullv ienqpv ideqpv /\
+    fifo_inv oemptyv ofullv oenqpv odeqpv /\
+    (if pinitRqv then NatLib.pow2 iaddrSize
+     else #pinitRqOfsv) =
+    #pinitRsOfsv +
+    fifoLength iemptyv ifullv ienqpv ideqpv +
+    fifoLength oemptyv ofullv oenqpv odeqpv.
 
   Definition fifo_empty_inv (fifoEmpty: bool) (fifoEnqP fifoDeqP: type (Bit fifoSize)): Prop :=
     fifoEmpty = true /\ fifoEnqP = fifoDeqP.
@@ -41,11 +109,13 @@ Section Invariants.
               evalExpr (getOptype _ rawInst) = opLd) /\
              (evalExpr (getOptype _ rawInst) = opLd ->
               (insElt insDeqP (RqFromProc !! "op") = false /\
-               evalExpr (getLdDst _ rawInst) <> (natToWord _ 0) /\
                insElt insDeqP (RqFromProc !! "addr") =
-               evalExpr (calcLdAddr
-                           _ (evalExpr (getLdAddr _ rawInst))
-                           (evalExpr (#rf@[getLdSrc _ rawInst])%kami_expr)) /\
+               evalExpr
+                 (alignLdAddr
+                    _ (evalExpr
+                         (calcLdAddr
+                            _ (evalExpr (getLdAddr _ rawInst))
+                            (evalExpr (#rf@[getLdSrc _ rawInst])%kami_expr)))) /\
                insElt insDeqP (RqFromProc !! "data") =
                evalConstT (getDefaultConst (Data dataBytes))))).
     - exact ((insElt insDeqP (RqFromProc !! "op") = true ->
@@ -59,16 +129,26 @@ Section Invariants.
                insElt insDeqP (RqFromProc !! "data") =
                evalExpr (#rf@[getStVSrc _ rawInst ])%kami_expr))).
   Defined.
-  Hint Unfold fifo_empty_inv fifo_not_empty_inv mem_request_inv: InvDefs.
+  Hint Unfold fifo_rq_rs_inv fifo_inv fifo_empty_inv fifo_not_empty_inv
+       mem_request_inv: InvDefs.
 
   Record procDec_inv (o: RegsT) : Prop :=
     { pcv : fullType type (SyntaxKind (Pc iaddrSize));
       Hpcv : M.find "pc"%string o = Some (existT _ _ pcv);
       rfv : fullType type (SyntaxKind (Vector (Data dataBytes) rfIdx));
       Hrfv : M.find "rf"%string o = Some (existT _ _ rfv);
+
+      pinitv : fullType type (SyntaxKind Bool);
+      Hpinitv : M.find "pinit"%string o = Some (existT _ _ pinitv);
+      pinitRqv : fullType type (SyntaxKind Bool);
+      HpinitRqv : M.find "pinitRq"%string o = Some (existT _ _ pinitRqv);
+      pinitRqOfsv : fullType type (SyntaxKind (Bit iaddrSize));
+      HpinitRqOfsv : M.find "pinitRqOfs"%string o = Some (existT _ _ pinitRqOfsv);
+      pinitRsOfsv : fullType type (SyntaxKind (Bit iaddrSize));
+      HpinitRsOfsv : M.find "pinitRsOfs"%string o = Some (existT _ _ pinitRsOfsv);
+      
       pgmv : fullType type (SyntaxKind (Vector (Data instBytes) iaddrSize));
       Hpgmv : M.find "pgm"%string o = Some (existT _ _ pgmv);
-
       stallv : fullType type (SyntaxKind Bool);
       Hstallv : M.find "stall"%string o = Some (existT _ _ stallv);
       iev : fullType type (SyntaxKind Bool);
@@ -92,18 +172,23 @@ Section Invariants.
       oeltv : fullType type (SyntaxKind (Vector (Struct RsToProc) fifoSize));
       Hoeltv : M.find "rsToProc"--"elt"%string o = Some (existT _ _ oeltv);
 
-      Hinv : or3
-               (stallv = false /\
-                fifo_empty_inv iev ienqpv ideqpv /\
-                fifo_empty_inv oev oenqpv odeqpv)
-               ((stallv = true /\
-                 fifo_not_empty_inv iev ienqpv ideqpv /\
-                 fifo_empty_inv oev oenqpv odeqpv) /\
-                (mem_request_inv (pgmv (split2 _ _ pcv)) rfv iev ieltv ideqpv))
-               (stallv = true /\
-                fifo_empty_inv iev ienqpv ideqpv /\
-                fifo_not_empty_inv oev oenqpv odeqpv)
-    }.
+      Hinv :
+        (pinitv = false ->
+         fifo_rq_rs_inv pinitRqv pinitRqOfsv pinitRsOfsv
+                        iev ifv oev ofv ienqpv ideqpv oenqpv odeqpv /\
+         stallv = false) /\
+        (pinitv = true ->
+         or3 (stallv = false /\
+              fifo_empty_inv iev ienqpv ideqpv /\
+              fifo_empty_inv oev oenqpv odeqpv)
+             ((stallv = true /\
+               fifo_not_empty_inv iev ienqpv ideqpv /\
+               fifo_empty_inv oev oenqpv odeqpv) /\
+              (mem_request_inv (pgmv (split2 _ _ pcv)) rfv iev ieltv ideqpv))
+             (stallv = true /\
+              fifo_empty_inv iev ienqpv ideqpv /\
+              fifo_not_empty_inv oev oenqpv odeqpv))
+        }.
 
   Ltac procDec_inv_old :=
     try match goal with
@@ -127,42 +212,269 @@ Section Invariants.
     | 2 => or3_thd (* responded *)
     end; intuition idtac.
 
+  Lemma fifoLength_enq:
+    forall emptyv enqpv deqpv,
+      fifo_inv emptyv false enqpv deqpv ->
+      fifoLength emptyv false enqpv deqpv + 1 =
+      fifoLength false (if weq deqpv (enqpv ^+ $1) then true else false)
+                 (enqpv ^+ $1) deqpv.
+  Proof.
+    unfold fifo_inv, fifoLength; intros.
+    destruct H.
+    destruct emptyv; simpl in *.
+    - specialize (H eq_refl); subst.
+      destruct (weq deqpv (deqpv ^+ $1)).
+      + destruct fifoSize; [reflexivity|].
+        exfalso; eapply wplus_one_neq; eauto.
+      + rewrite wminus_def, <-wplus_assoc.
+        rewrite wplus_comm with (x:= $1).
+        rewrite wplus_assoc.
+        rewrite wminus_inv, wplus_wzero_2.
+        destruct fifoSize.
+        * elim n.
+          rewrite (word0 deqpv); reflexivity.
+        * rewrite roundTrip_1; reflexivity.
+    - destruct (weq deqpv (enqpv ^+ $1)); subst.
+      + rewrite wminus_def, wneg_wplus_distr.
+        rewrite wplus_assoc, wminus_inv, wplus_wzero_2.
+        destruct fifoSize; [reflexivity|].
+        rewrite <-wones_wneg_one.
+        rewrite wones_pow2_minus_one.
+        pose proof (NatLib.pow2_zero (S n)); omega.
+      + rewrite wminus_def with (x:= enqpv ^+ _).
+        rewrite <-wplus_assoc, wplus_comm with (x:= $1).
+        rewrite wplus_assoc, <-wminus_def.
+        erewrite wordToNat_plusone with (w':= wones _).
+        * omega.
+        * apply lt_wlt.
+          pose proof (wordToNat_bound (enqpv ^- deqpv)).
+          rewrite wones_pow2_minus_one.
+          assert (#(enqpv ^- deqpv) <> NatLib.pow2 fifoSize - 1).
+          { intro Hx.
+            rewrite <-wones_pow2_minus_one in Hx.
+            assert (enqpv ^- deqpv = wones fifoSize).
+            { rewrite <-natToWord_wordToNat, <-Hx.
+              rewrite natToWord_wordToNat; reflexivity.
+            }
+            assert (^~ (enqpv ^- deqpv) = $1).
+            { rewrite H2, <-wneg_idempotent with (w:= $1).
+              rewrite wones_wneg_one; reflexivity.
+            }
+            elim n.
+            rewrite <-H3.
+            rewrite wminus_def, wneg_wplus_distr.
+            rewrite wplus_assoc, wneg_idempotent.
+            rewrite wminus_inv, wplus_wzero_2.
+            reflexivity.
+          }
+          omega.
+  Qed.
+
+  Lemma fifoLength_deq:
+    forall fullv enqpv deqpv,
+      fifo_inv false fullv enqpv deqpv ->
+      fifoLength false fullv enqpv deqpv =
+      fifoLength (if weq enqpv (deqpv ^+ $1) then true else false) false 
+                 enqpv (deqpv ^+ $1) + 1.
+  Proof.
+    unfold fifo_inv, fifoLength; intros.
+    destruct H.
+    destruct fullv; simpl in *.
+    - specialize (H eq_refl); subst.
+      destruct (weq deqpv (deqpv ^+ $1)).
+      + destruct fifoSize; [reflexivity|].
+        exfalso; eapply wplus_one_neq; eauto.
+      + rewrite wminus_def, wneg_wplus_distr.
+        rewrite wplus_assoc, wminus_inv, wplus_wzero_2.
+        rewrite <-wones_wneg_one.
+        rewrite wones_pow2_minus_one.
+        pose proof (NatLib.pow2_zero fifoSize); omega.
+    - destruct (weq enqpv (deqpv ^+ $1)).
+      + subst.
+        rewrite wminus_def, <-wplus_assoc.
+        rewrite wplus_comm with (x:= $1).
+        rewrite wplus_assoc.
+        rewrite wminus_inv, wplus_wzero_2.
+        destruct fifoSize.
+        * rewrite (word0 deqpv) in H0.
+          specialize (H0 eq_refl); discriminate.
+        * rewrite roundTrip_1; reflexivity.
+      + rewrite wminus_plus_distr.
+        rewrite <-wordToNat_minus_one'.
+        * omega.
+        * intro Hx.
+          apply sub_0_eq in Hx; subst.
+          specialize (H0 eq_refl); discriminate.
+  Qed.
+
+  Lemma fifoLength_zero:
+    forall emptyv fullv enqpv deqpv,
+      fifo_inv emptyv fullv enqpv deqpv ->
+      fifoLength emptyv fullv enqpv deqpv = 0 ->
+      emptyv = true /\ enqpv = deqpv.
+  Proof.
+    unfold fifo_inv, fifoLength; intros.
+    destruct emptyv.
+    - destruct H; specialize (H eq_refl); subst; auto.
+    - destruct fullv.
+      + pose proof (NatLib.pow2_zero fifoSize); omega.
+      + exfalso.
+        rewrite <-wordToNat_wzero with (sz:= fifoSize) in H0.
+        assert (enqpv ^- deqpv = wzero fifoSize).
+        { rewrite <-natToWord_wordToNat, <-H0.
+          rewrite natToWord_wordToNat.
+          reflexivity.
+        }
+        apply sub_0_eq in H1; subst.
+        destruct H; specialize (H1 eq_refl); discriminate.
+  Qed.
+
+  Lemma fifoLength_one:
+    forall fullv enqpv deqpv,
+      fifo_inv false fullv enqpv deqpv ->
+      fifoLength false fullv enqpv deqpv = 1 ->
+      fifoSize = 0 \/ enqpv = deqpv ^+ $1.
+  Proof.
+    unfold fifo_inv, fifoLength; intros.
+    destruct fifoSize; [left; reflexivity|].
+    destruct fullv.
+    - exfalso; pose proof (NatLib.one_lt_pow2 n); omega.
+    - right.
+      rewrite wplus_comm.
+      apply wminus_wplus_transpose.
+      rewrite <-natToWord_wordToNat with (w:= enqpv ^- deqpv).
+      congruence.
+  Qed.
+
+  Lemma fifoLength_not_empty:
+    forall fullv enqpv deqpv,
+      fifo_inv false fullv enqpv deqpv ->
+      (fifoLength false fullv enqpv deqpv > 0)%nat.
+  Proof.
+    unfold fifo_inv, fifoLength; intros.
+    destruct fullv.
+    - apply NatLib.pow2_zero.
+    - apply gt0_wneq0.
+      intro Hx.
+      apply wminus_wplus_transpose in Hx.
+      rewrite wplus_wzero_2 in Hx; subst.
+      destruct H; specialize (H0 eq_refl).
+      discriminate.
+  Qed.
+
+  Lemma fifo_rq_rs_inv_last:
+    forall (pinitRqv: type Bool) (pinitRqOfsv: type (Bit iaddrSize))
+           iev ifv ienqpv ideqpv ofv oenqpv odeqpv,
+      fifo_inv iev ifv ienqpv ideqpv ->
+      fifo_inv false ofv oenqpv odeqpv ->
+      (if pinitRqv then NatLib.pow2 iaddrSize else # (pinitRqOfsv)) =
+      (NatLib.pow2 iaddrSize - 1) +
+      fifoLength iev ifv ienqpv ideqpv +
+      fifoLength false ofv oenqpv odeqpv ->
+      pinitRqv = true /\
+      iev = true /\ (* ifv = false /\ *) ienqpv = ideqpv /\
+      oenqpv = odeqpv ^+ $1.
+  Proof.
+    intros.
+    pose proof (fifoLength_not_empty H0).
+    find_if_inside;
+      [|exfalso; pose proof (wordToNat_bound pinitRqOfsv); omega].
+
+    assert (fifoLength iev ifv ienqpv ideqpv = 0) by omega.
+    apply fifoLength_zero in H3; [|assumption].
+    dest; subst.
+
+    assert (fifoLength false ofv oenqpv odeqpv = 1) by omega.
+    apply fifoLength_one in H3; [|assumption].
+    destruct H3.
+    - clear -H3; subst.
+      repeat split.
+      rewrite (word0 oenqpv), (word0 odeqpv); reflexivity.
+    - subst; repeat split.
+  Qed.
+
   Lemma procDec_inv_ok':
     forall init n ll,
       init = initRegs (getRegInits (fst pdecInl)) ->
       Multistep (fst pdecInl) init n ll ->
       procDec_inv n.
-  Proof. (* SKIP_PROOF_ON
+  Proof. (* SKIP_PROOF_OFF *)
     induction 2.
 
     - kinv_dest_custom procDec_inv_tac.
-      procDec_inv_next 0.
+      kinv_constr.
+      + cbn; repeat rewrite wordToNat_wzero; split; intros; reflexivity.
+      + cbn; repeat rewrite wordToNat_wzero; split; intros; reflexivity.
+      + cbn; repeat rewrite wordToNat_wzero; reflexivity.
+      + procDec_inv_next 0.
 
-    - kinvert.
-      + mred.
-      + mred.
-      + kinv_dest_custom procDec_inv_tac.
-        procDec_inv_next 1; kinv_eq; kinv_finish.
-      + kinv_dest_custom procDec_inv_tac.
-        procDec_inv_next 0.
-      + kinv_dest_custom procDec_inv_tac.
-        procDec_inv_next 1; kinv_eq; kinv_finish.
-      + kinv_dest_custom procDec_inv_tac.
-        procDec_inv_next 0.
-      + kinv_dest_custom procDec_inv_tac.
-        procDec_inv_next 0.
-      + kinv_dest_custom procDec_inv_tac.
-        procDec_inv_next 0.
-      + kinv_dest_custom procDec_inv_tac.
-        procDec_inv_next 0.
-      + kinv_dest_custom procDec_inv_tac.
-        procDec_inv_next 0.
-      + kinv_dest_custom procDec_inv_tac.
-        procDec_inv_next 2.
-      + kinv_dest_custom procDec_inv_tac.
-        procDec_inv_next 2.
+    - kinvert; [mred|mred|..].
+      + kinv_dest_custom procDec_inv_tac; kinv_constr.
+        * split; intros.
+          { rewrite orb_false_l in H2; find_if_inside; [auto|discriminate]. }
+          { rewrite orb_false_l; find_if_inside; [reflexivity|exfalso; auto]. }
+        * assumption.
+        * rewrite wnot_not_zero_wplusone by assumption.
+          erewrite <-fifoLength_enq with (emptyv:= iev) by (apply H; auto).
+          omega.
 
-        END_SKIP_PROOF_ON *) apply cheat.
+      + kinv_dest_custom procDec_inv_tac; kinv_constr.
+        * split; intros.
+          { rewrite orb_false_l in H2; find_if_inside; [auto|discriminate]. }
+          { rewrite orb_false_l; find_if_inside; [reflexivity|exfalso; auto]. }
+        * assumption.
+        * erewrite <-fifoLength_enq with (emptyv:= iev) by (apply H; auto).
+          replace #x1 with (NatLib.pow2 iaddrSize - 1) in H4.
+          { pose proof (NatLib.pow2_zero iaddrSize); omega. }
+          { replace x1 with (wones iaddrSize).
+            { apply eq_sym, wones_pow2_minus_one. }
+            { apply wnot_zero_wones in e; auto. }
+          }
+
+      + kinv_dest_custom procDec_inv_tac; kinv_constr.
+        * assumption.
+        * split; intros.
+          { rewrite orb_false_r in H2; find_if_inside; [auto|discriminate]. }
+          { rewrite orb_false_r; find_if_inside; [reflexivity|exfalso; auto]. }
+        * rewrite wnot_not_zero_wplusone by assumption.
+          rewrite fifoLength_deq in H4 by (apply H3; auto).
+          omega.
+          
+      + kinv_dest_custom procDec_inv_tac; kinv_constr.
+        apply wnot_zero_wones in e; subst.
+        rewrite wones_pow2_minus_one in H4.
+        eapply fifo_rq_rs_inv_last in H4; [|assumption|assumption].
+        dest; subst.
+        procDec_inv_next 0; kinv_finish.
+
+      + kinv_dest_custom procDec_inv_tac; kinv_constr.
+        procDec_inv_next 1; kinv_eq; kinv_finish.
+      + kinv_dest_custom procDec_inv_tac; kinv_constr.
+        procDec_inv_next 1; kinv_eq; kinv_finish.
+      + kinv_dest_custom procDec_inv_tac; kinv_constr.
+        procDec_inv_next 0.
+      + kinv_dest_custom procDec_inv_tac; kinv_constr.
+        procDec_inv_next 0.
+      + kinv_dest_custom procDec_inv_tac; kinv_constr.
+        procDec_inv_next 0.
+      + kinv_dest_custom procDec_inv_tac; kinv_constr.
+        procDec_inv_next 0.
+      + kinv_dest_custom procDec_inv_tac; kinv_constr.
+        procDec_inv_next 0.
+      + kinv_dest_custom procDec_inv_tac; kinv_constr.
+        * split; intros.
+          { rewrite orb_false_r in H2; find_if_inside; [assumption|discriminate]. }
+          { rewrite orb_false_r; find_if_inside; [reflexivity|exfalso; auto]. }
+        * split; intros.
+          { rewrite orb_false_l in H2; find_if_inside; [auto|discriminate]. }
+          { rewrite orb_false_l; find_if_inside; [reflexivity|exfalso; auto]. }
+        * erewrite <-fifoLength_enq with (emptyv:= oev) by assumption.
+          rewrite Nat.add_comm with (m:= 1), Nat.add_assoc.
+          rewrite <-Nat.add_assoc with (n:= #pinitRsOfsv).
+          erewrite <-fifoLength_deq with (fullv:= ifv) by assumption.
+          assumption.
+        * procDec_inv_old; procDec_inv_next 2.
+          (* END_SKIP_PROOF_OFF *)
   Qed.
 
   Lemma procDec_inv_ok:
@@ -177,5 +489,6 @@ Section Invariants.
 End Invariants.
 
 Hint Unfold RqFromProc RsToProc: MethDefs.
-Hint Unfold fifo_empty_inv fifo_not_empty_inv mem_request_inv: InvDefs.
+Hint Unfold fifo_rq_rs_inv fifo_inv fifo_empty_inv fifo_not_empty_inv
+       mem_request_inv: InvDefs.
     
